generational/spec/GC.Gen.CheneyPreservation.fsti
@@ -113,7 +113,7 @@ val cheney_promote_preserves_no_scan_invariant
 val cheney_promote_preserves_blue_fields_closed
   (minor: minor_state) (major: heap) (fp: U64.t) (roots: seq U64.t)
   : Lemma (requires well_formed_heap major /\
-                    no_infix_field_targets major /\
+                    blue_fields_non_infix major /\
                     AllocLemmas.fl_valid major fp heap_words /\
                     AllocLemmas.fl_chain_terminates major fp heap_words /\
                     chain_objects_blue major fp /\
@@ -328,7 +328,7 @@ val cheney_collect_preserves_wfh_from_shape
     (requires GenInv.collection_heap_shape minor major fp)
     (ensures well_formed_heap
       (cheney_collect_spec minor major fp roots).mc_major /\
-      no_infix_field_targets
+      blue_fields_non_infix
       (cheney_collect_spec minor major fp roots).mc_major)
 
 val cheney_collect_preserves_no_pointer_to_blue
